src/QuasiSeq.v
@@ -1,0 +1,306 @@
+Require Import Bool List String Peano_dec.
+Require Import Common ListSupport FMap Syntax Semantics StepM StepT SemFacts.
+Require Import Serial SerialFacts Reduction.
+
+Require Import Omega Wf.
+
+Set Implicit Arguments.
+
+(*! Quasi-sequential histories *)
+
+Section QuasiSeq.
+  Variables (sys: System)
+            (quasiSeq: forall (sys: System) (hst: MHistory) (n: nat), Prop).
+
+  Definition QuasiSeqOkInit :=
+    forall hst st,
+      steps step_m sys (initsOf sys) hst st ->
+      exists n, quasiSeq sys hst n.
+
+  Definition QuasiSeqOkStep :=
+    forall hst st n,
+      steps step_m sys (initsOf sys) hst st ->
+      quasiSeq sys hst n ->
+      ((exists trss, Sequential sys msg_dec hst trss) \/
+       (exists rhst m, Reduced sys hst rhst /\
+                       quasiSeq sys rhst m /\ m < n)).
+
+  Lemma quasiSeq_implies_serializableSys:
+    QuasiSeqOkStep ->
+    forall n hst st,
+      steps step_m sys (initsOf sys) hst st ->
+      quasiSeq sys hst n ->
+      Serializable sys hst.
+  Proof.
+    induction n as [n IHn] using (well_founded_induction lt_wf).
+    intros.
+    specialize (H _ _ _ H0 H1); destruct H; dest.
+    - eapply sequential_serializable; eauto.
+    - eapply reduced_serializable; eauto.
+      eapply IHn; eauto.
+      eapply H; eauto.
+  Qed.
+
+  Lemma quasiSeqOk_implies_serializableSys:
+    QuasiSeqOkInit -> QuasiSeqOkStep -> SerializableSys sys.
+  Proof.
+    intros; red; intros.
+    specialize (H _ _ H1); destruct H as [n ?].
+    eapply quasiSeq_implies_serializableSys; eauto.
+  Qed.
+
+End QuasiSeq.
+
+(*! Semi-sequential (as quasi-sequential) histories *)
+
+(* The number of [STransactional] segments is the decreasing factor when
+ * defining [SSequential] as a predicate for quasi-sequential histories.
+ *
+ * In a bird's eye view, how do we know that number is decreasing?
+ * 0) For a given legal history [hst], always [exists n, SSequential hst n]
+ * 1) When a history is semi-sequential, 
+ *    it's either [Sequential] or [Interleaved]
+ * 2) If a history is [Interleaved], then it's [MinInterleaved].
+ * 3) Let [hst1] and [hst2] be minimally-interleaving sequences in [hst].
+ *    [WellInterleaved] says that [hst1] and [hst2] can be merged by a number
+ *    of reductions.
+ * 4) [WellInterleaved] directly implies [Serializable].
+ *)
+
+Definition Continuous (hst1 hst2: MHistory) :=
+  exists inits1 ins1 outs1 eouts1 inits2 ins2 outs2 eouts2,
+    Atomic msg_dec inits1 ins1 hst1 outs1 eouts1 /\
+    Atomic msg_dec inits2 ins2 hst2 outs2 eouts2 /\
+    inits2 <> nil /\
+    SubList inits2 eouts1.
+
+Definition Separated (hsts: list MHistory) :=
+  forall hst1 hst2 hsts1 hsts2 hsts3,
+    hsts = hsts3 ++ hst2 :: hsts2 ++ hst1 :: hsts1 ->
+    ~ Continuous hst1 hst2.
+
+Definition Interleaved (hsts: list MHistory) :=
+  exists hst1 hst2 hsts1 hsts2 hsts3,
+    hsts = hsts3 ++ hst2 :: hsts2 ++ hst1 :: hsts1 /\
+    Continuous hst1 hst2.
+
+Definition MinInterleaved (hsts: list MHistory) :=
+  exists hst1 hst2 hsts1 hsts2 hsts3,
+    hsts = hsts3 ++ hst2 :: hsts2 ++ hst1 :: hsts1 /\
+    Continuous hst1 hst2 /\
+    Separated (hsts2 ++ [hst1]) /\
+    Separated (hst2 :: hsts2).
+
+Lemma interleaved_min:
+  forall hsts, Interleaved hsts -> MinInterleaved hsts.
+Proof.
+Admitted.
+
+Lemma separated_cons:
+  forall (hsts1 hsts2: list MHistory) hst,
+    Separated (hsts2 ++ hst :: hsts1) ->
+    Forall (fun phst => ~ Continuous phst hst) hsts1 /\
+    Forall (fun nhst => ~ Continuous hst nhst) hsts2 /\
+    Separated (hsts2 ++ hsts1).
+Proof.
+Admitted.
+
+Lemma continuous_atomic_concat:
+  forall (hst1 hst2: MHistory),
+    Continuous hst1 hst2 ->
+    exists inits ins outs eouts,
+      Atomic msg_dec inits ins (hst2 ++ hst1) outs eouts.
+Proof.
+  unfold Continuous; intros; dest.
+  pose proof (atomic_app H H1 H0 H2); dest.
+  eauto.
+Qed.
+
+Lemma stransactional_sequential_or_interleaved:
+  forall sys trss st,
+    steps step_m sys (initsOf sys) (List.concat trss) st ->
+    Forall (STransactional msg_dec) trss ->
+    Sequential sys msg_dec (List.concat trss) trss \/
+    Interleaved trss.
+Proof.
+  induction trss as [|trs trss]; simpl; intros;
+    [left; constructor; auto|].
+
+  eapply steps_split in H; [|reflexivity].
+  destruct H as [sti [? ?]].
+  inv H0.
+  specialize (IHtrss _ H H5); destruct IHtrss.
+
+  - (* TODO: need to prove that whenever a semi-transaction
+     * [STransactional ins trs outs] is added to a history ([List.concat trss]),
+     * [ins] is either a new semi-transaction or a continuation from one of 
+     * previous semi-transactions.
+     *
+     * This is not true when [ins] takes a part from [trs1] and the other part
+     * from [trs2], where [trs1 <> trs2] and [trs1 ∈ trss /\ trs2 ∈ trss].
+     * Thus we need a static condition to ensure each rule in the system takes
+     * incoming messages for a single transaction.
+     *)
+    admit.
+  - right.
+    clear -H0.
+    destruct H0 as [hst1 [hst2 [hsts1 [hsts2 [hsts3 [? ?]]]]]]; subst.
+    exists hst1, hst2, hsts1, hsts2, (trs :: hsts3).
+    split; auto.
+Admitted.
+
+Section WellInterleaved.
+  Variable (sys: System).
+
+  Definition WellInterleaved :=
+    forall hst1 hst2,
+      Continuous hst1 hst2 ->
+      forall hsts,
+        Forall (STransactional msg_dec) hsts ->
+        Separated (hsts ++ [hst1]) ->
+        Separated (hst2 :: hsts) ->
+        exists rhst1 rhst2,
+          Reduced sys (List.concat (hst2 :: hsts ++ [hst1]))
+                  (List.concat (rhst2 ++ hst2 :: hst1 :: rhst1)) /\
+          Forall (STransactional msg_dec) (rhst2 ++ rhst1) /\
+          List.length hsts = List.length (rhst2 ++ rhst1).
+
+  Lemma well_interleaved_reduced:
+    forall (Hwi: WellInterleaved) trss st1 st2,
+      steps step_m sys st1 (List.concat trss) st2 ->
+      Forall (STransactional msg_dec) trss ->
+      Interleaved trss ->
+      exists (rhst : MHistory) (m : nat),
+        Reduced sys (List.concat trss) rhst /\
+        SSequential msg_dec rhst m /\
+        m < Datatypes.length trss.
+  Proof.
+    intros.
+    apply interleaved_min in H1.
+    destruct H1 as [hst1 [hst2 [hsts1 [hsts2 [hsts3 [? [? [? ?]]]]]]]]; subst.
+    match goal with
+    | [H: steps step_m _ _ ?hst _ |- _] =>
+      replace hst with ((List.concat hsts3)
+                          ++ (List.concat (hst2 :: hsts2 ++ [hst1]))
+                          ++ (List.concat hsts1)) in *;
+        [|simpl; repeat rewrite <-app_assoc;
+          repeat rewrite concat_app; simpl;
+          rewrite <-app_assoc, app_nil_r;
+          repeat rewrite concat_app; simpl;
+          reflexivity]
+    end.
+    eapply steps_split in H; [|reflexivity]; destruct H as [sti2 [? ?]].
+    eapply steps_split in H; [|reflexivity]; destruct H as [sti1 [? ?]].
+    apply Forall_app_inv in H0; dest.
+    inv H6; apply Forall_app_inv in H10; dest; inv H7.
+    pose proof (Hwi _ _ H2 _ H6 H3 H4).
+    destruct H7 as [rhst1 [rhst2 [? [? ?]]]].
+
+    exists ((List.concat hsts3)
+              ++ (List.concat (rhst2 ++ (hst2 ++ hst1) :: rhst1))
+              ++ (List.concat hsts1)); eexists.
+    split; [|split].
+    - apply reduced_app_1.
+      apply reduced_app_2.
+      replace (List.concat (rhst2 ++ (hst2 ++ hst1) :: rhst1))
+        with (List.concat (rhst2 ++ hst2 :: hst1 :: rhst1)); [assumption|].
+      repeat (rewrite concat_app; simpl).
+      rewrite <-app_assoc; reflexivity.
+    - econstructor.
+      + repeat rewrite <-concat_app; reflexivity.
+      + reflexivity.
+      + apply Forall_app_inv in H8; dest.
+        repeat (apply Forall_app; auto).
+        constructor; auto.
+        eapply continuous_atomic_concat in H2; eauto.
+        destruct H2 as [inits [ins [outs [eouts ?]]]].
+        eapply STrsAtomic; eauto.
+    - repeat (simpl; try rewrite app_length).
+      unfold MHistory; rewrite H10.
+      apply plus_lt_compat_l.
+      rewrite app_length.
+      rewrite <-Nat.add_assoc; simpl.
+      repeat rewrite Nat.add_succ_r.
+      rewrite Nat.add_assoc.
+      auto.
+  Qed.
+
+  Definition WellInterleavedInd :=
+    forall hst1 hst2,
+      Continuous hst1 hst2 ->
+      forall hst,
+        STransactional msg_dec hst ->
+        forall hsts,
+          Forall (STransactional msg_dec) hsts ->
+          Forall (fun phst => ~ Continuous phst hst) (hsts ++ [hst1]) ->
+          ~ Continuous hst hst2 ->
+          Reduced sys (hst2 ++ hst ++ List.concat hsts ++ hst1)
+                  (hst2 ++ List.concat hsts ++ hst1 ++ hst) \/
+          Reduced sys (hst2 ++ hst ++ List.concat hsts ++ hst1)
+                  (hst ++ hst2 ++ List.concat hsts ++ hst1).
+
+  Lemma well_interleaved_ind_ok:
+    forall (Hwii: WellInterleavedInd), WellInterleaved.
+  Proof.
+    red; induction hsts as [|hst hsts]; simpl; intros;
+      [exists nil, nil; simpl; split; auto; apply reduced_refl|].
+
+    inv H0.
+
+    apply separated_cons with (hsts2:= nil) in H1; dest; simpl in *; clear H1.
+    apply separated_cons with (hsts2:= [hst2]) in H2; dest.
+    inv H2; clear H10.
+    
+    specialize (IHhsts H6 H3 H4).
+    destruct IHhsts as [rhst1 [rhst2 ?]]; dest.
+
+    eapply Hwii in H6; eauto.
+    specialize (H6 H0 H9).
+    destruct H6.
+    - exists (rhst1 ++ [hst]), rhst2.
+      split; [|split].
+      + repeat (simpl; try rewrite concat_app; try rewrite app_nil_r).
+        repeat (simpl in H2; try rewrite concat_app in H2; try rewrite app_nil_r in H2).
+        eapply reduced_trans; [eassumption|].
+        repeat rewrite app_assoc.
+        apply reduced_app_2.
+        repeat rewrite <-app_assoc.
+        assumption.
+      + apply Forall_app_inv in H7; dest.
+        repeat apply Forall_app; eauto.
+      + repeat rewrite app_length.
+        rewrite app_length in H8.
+        rewrite Nat.add_assoc, <-H8.
+        simpl; omega.
+    - exists rhst1, (hst :: rhst2).
+      split; [|split].
+      + repeat (simpl; try rewrite concat_app; try rewrite app_nil_r).
+        repeat (simpl in H2; try rewrite concat_app in H2; try rewrite app_nil_r in H2).
+        eapply reduced_trans; [eassumption|].
+        apply reduced_app_1.
+        assumption.
+      + apply Forall_app_inv in H7; dest.
+        repeat apply Forall_app; eauto.
+      + simpl; rewrite app_length.
+        rewrite app_length in H8.
+        rewrite <-H8.
+        auto.
+  Qed.
+
+  Lemma well_interleaved_serializable:
+    WellInterleaved -> SerializableSys sys.
+  Proof.
+    intros.
+    apply quasiSeqOk_implies_serializableSys
+      with (quasiSeq := fun _ hst n => SSequential msg_dec hst n).
+    - red; intros.
+      apply ssequential_default.
+    - red; intros.
+      inv H1.
+      pose proof (stransactional_sequential_or_interleaved H0 H4).
+      destruct H1; eauto.
+      right; eapply well_interleaved_reduced; eauto.
+  Qed.
+
+End WellInterleaved.
+
